theories/misc_unused/hoInterps_experiments.v
@@ -6,6 +6,7 @@ From iris.base_logic Require Import lib.saved_prop.
 From D Require Import iris_prelude.
 From D Require Import saved_interp_dep asubst_intf asubst_base dlang lty.
 From D Require Import swap_later_impl.
+From D.Dot Require dot_lty unary_lr.
 
 Import EqNotations.
 
@@ -44,49 +45,161 @@ Definition hoLtyO Σ n := vec vl n -d> ltyO Σ.
 Definition envApply {Σ n} : oltyO Σ n → env → hoLtyO Σ n :=
   λ T, flip T.
 
-Definition oCurry {n} {A : ofeT} (Φ : vec vl (S n) → A) :
+Definition oCurry {n} {A : ofeT} (Φ : vec vl n.+1 → A) :
   vl -d> vec vl n -d> A := vcurry Φ.
 
 Definition oUncurry {n} {A : ofeT} (Φ : vl → vec vl n → A) :
-  vec vl (S n) -d> A := vuncurry Φ.
+  vec vl n.+1 -d> A := vuncurry Φ.
 Definition oLaterN {Σ n} i (τ : olty Σ n) := Olty (eLater i τ).
 
-Inductive skind {Σ} : nat → Type :=
-  | skintv : olty Σ 0 → olty Σ 0 → skind 0
-  | skpi n : olty Σ 0 → skind n → skind (S n).
-Global Arguments skind: clear implicits.
+(** An inductive representation of gHkDOT semantic kinds. *)
+Inductive s_kind {Σ} : nat → Type :=
+  | s_kintv : olty Σ 0 → olty Σ 0 → s_kind 0
+  | s_kpi n : olty Σ 0 → s_kind n → s_kind n.+1.
+Global Arguments s_kind: clear implicits.
 
-Record spine_skind {Σ} {n : nat} : Type := SpineSK {
+(** Alternative inductive representation of gHkDOT semantic kinds. *)
+Record spine_s_kind {Σ} {n : nat} : Type := SpineSK {
   spine_kargs : vec (olty Σ 0) n;
   spine_L : olty Σ 0;
   spine_U : olty Σ 0;
 }.
-Arguments spine_skind : clear implicits.
+Arguments spine_s_kind : clear implicits.
 
-Section saved_ho_sem_type_extra.
+(** Semantic kinds can be interpreted into predicates. *)
+(** Semantic Kinds as unary Predicates. *)
+Notation sp_kind Σ n := (env → hoLty Σ n → iProp Σ).
+(** Semantic Kinds as relations. *)
+Notation sr_kind Σ n := (env → hoLtyO Σ n → hoLtyO Σ n → iProp Σ).
+
+Notation iRel P Σ := (P Σ → P Σ → iProp Σ).
+Definition subtype_lty {Σ} : iRel ltyO Σ := λI φ1 φ2,
+  □ ∀ v, φ1 v → φ2 v.
+
+Infix "⊆" := subtype_lty : bi_scope.
+Notation "X ⊆ Y ⊆ Z" := (X ⊆ Y ∧ Y ⊆ Z)%I : bi_scope.
+Notation "X ⊆ Y ⊆ Z ⊆ W" := (X ⊆ Y ∧ Y ⊆ Z ∧ Z ⊆ W)%I (at level 70, Y, Z at next level) : bi_scope.
+
+(** Semantic Full Kind. *)
+Record sf_kind {Σ n} := Sfkind {
+  sf_kind_car :> sp_kind Σ n;
+  sf_kind_sub : sr_kind Σ n;
+}.
+Global Arguments sf_kind : clear implicits.
+Global Arguments sf_kind_car : simpl never.
+Global Arguments sf_kind_sub : simpl never.
+
+Section kinds_types.
   Context {Σ}.
 
-  Definition sp_skintv (L U : olty Σ 0) : spine_skind Σ 0 := SpineSK vnil L U.
-  Definition sp_skpi {n} (S : olty Σ 0) (K : spine_skind Σ n) : spine_skind Σ n.+1 :=
+  Definition sp_intv (L U : olty Σ 0) : spine_s_kind Σ 0 := SpineSK vnil L U.
+  Definition sp_pi {n} (S : olty Σ 0) (K : spine_s_kind Σ n) : spine_s_kind Σ n.+1 :=
     SpineSK (vcons S (spine_kargs K)) (spine_L K) (spine_U K).
 
-  Fixpoint skind_to_spine_skind {n} (K : skind Σ n) : spine_skind Σ n :=
+  Definition sf_intv (L U : olty Σ 0) : sf_kind Σ 0 :=
+    Sfkind
+      (λI ρ φ,
+        oClose L ρ ⊆ oClose φ ⊆ oClose U ρ)
+      (λI ρ φ1 φ2,
+        oClose L ρ ⊆ oClose φ1 ⊆ oClose φ2 ⊆ oClose U ρ).
+
+  Definition sf_pi {n} (S : olty Σ 0) (K : sf_kind Σ n) : sf_kind Σ n.+1 :=
+    Sfkind
+      (λI ρ φ,
+        □∀ arg, oClose S ρ arg →
+        sf_kind_car K (arg .: ρ) (vcurry φ arg))
+      (λI ρ φ1 φ2,
+        □∀ arg, oClose S ρ arg →
+        sf_kind_sub K (arg .: ρ) (vcurry φ1 arg) (vcurry φ2 arg)).
+
+
+  Definition sf_star : sf_kind Σ 0 := sf_intv oBot oTop.
+
+  Fixpoint s_kind_to_spine_s_kind {n} (K : s_kind Σ n) : spine_s_kind Σ n :=
     match K with
-    | skintv L U => sp_skintv L U
-    | skpi s K => sp_skpi s (skind_to_spine_skind K)
+    | s_kintv L U => sp_intv L U
+    | s_kpi s K => sp_pi s (s_kind_to_spine_s_kind K)
     end.
 
-End saved_ho_sem_type_extra.
+  Definition spine_s_kind_to_sf_kind {n} (K : spine_s_kind Σ n) : sf_kind Σ n :=
+    vec_fold (sf_intv (spine_L K) (spine_U K)) (@sf_pi) n (spine_kargs K).
+  Global Arguments spine_s_kind_to_sf_kind {_} !_.
+
+  Fixpoint s_kind_to_sf_kind {n} (K : s_kind Σ n) : sf_kind Σ n :=
+    match K with
+    | s_kintv L U => sf_intv L U
+    | s_kpi s K => sf_pi s (s_kind_to_sf_kind K)
+    end.
+
+  Lemma s_kind_refl {n} (K : s_kind Σ n) T (ρ : env) :
+    let sfK := s_kind_to_sf_kind K in
+    sfK ρ T -∗ sf_kind_sub sfK ρ T T.
+  Proof.
+    elim: n ρ K T => [|n IHn] ρ; cbn.
+    - move E: 0 => n K T. destruct K eqn:?; simplify_eq.
+      by iIntros "($&$) !>" (v) "$".
+    - move E: n.+1 => m K T.
+      (* case E': K T E => [|m S K'].
+      case: K T E. admit. *)
+      destruct K as [|m S K'] eqn:?; simplify_eq/=.
+      iIntros "#H !>" (arg) "#Harg".
+      iApply IHn.
+      iApply ("H" with "Harg").
+  Qed.
+
+  Definition oLam {n} (τ : oltyO Σ n) : oltyO Σ n.+1 :=
+    Olty (λ args ρ, τ (vtail args) (vhead args .: ρ)).
+    (* vuncurry (λ v, Olty (λ args ρ, τ args (v .: ρ))). *)
+  Definition oTAppV {n} (τ : oltyO Σ n.+1) v : olty Σ n := vcurry τ v.
+
+  Lemma swap_oLam_oLater {n} (τ : olty Σ n) :
+    oLater (oLam τ) ≡ oLam (oLater τ).
+  Proof. done. Qed.
+
+  Lemma swap_oTApp_oLater {n} (τ : olty Σ (S n)) v:
+    oLater (oTAppV τ v) ≡ oTAppV (oLater τ) v.
+  Proof. done. Qed.
+
+End kinds_types.
+
+(** Kinded, indexed subtyping *)
+Program Definition sstpk `{!dlangG Σ} {n} i j Γ T1 T2 (K : sf_kind Σ n) : iProp Σ :=
+  □∀ ρ, s⟦Γ⟧*ρ → sf_kind_sub K ρ (envApply (oLaterN i T1) ρ) (envApply (oLaterN j T2) ρ).
+Notation "Γ s⊨ T1 , i <: T2 , j ∷ K" := (sstpk i j Γ T1 T2 K)
+  (at level 74, i, j, T1, T2, K at next level).
+Definition sktp `{!dlangG Σ} {n} i Γ T (K : sf_kind Σ n) : iProp Σ :=
+  □∀ ρ, s⟦Γ⟧*ρ → ▷^i K ρ T.
+Notation "Γ s⊨ T ∷[ i ] K" := (sktp i Γ T K)
+  (at level 74, T, K at next level).
+Definition ssktp `{!dlangG Σ} {n} i Γ (K1 K2 : sf_kind Σ n) : iProp Σ :=
+  □∀ ρ (T : olty Σ n), s⟦Γ⟧*ρ → ▷^i (K1 ρ (envApply T ρ) → K2 ρ (envApply T ρ)).
+Notation "Γ s⊨ K1 <∷[ i ] K2" := (ssktp i Γ K1 K2)
+  (at level 74, K1, K2 at next level).
+
 End HoSemTypes.
 
-From D.Dot Require Import dot_lty unary_lr.
-
+Module HkDot.
+Import dot_lty unary_lr.
+Include HoSemTypes VlSorts dlang_inst dot_lty.
 Implicit Types
          (v w : vl) (e : tm) (d : dm) (ds : dms) (p : path)
-         (vs : vls) (ρ : var → vl) (l : label).
+         (ρ : var → vl) (l : label).
 
-Module HkDot.
-Include HoSemTypes VlSorts dlang_inst dot_lty.
+Section dot_types.
+  Context `{dlangG Σ} `{HswapProp: SwapPropI Σ}.
 
+  Lemma sstpk_star_eq_sstp Γ i j T1 T2 :
+    Γ s⊨ T1 , i <: T2 , j ∷ sf_star ⊣⊢ Γ s⊨ T1 , i <: T2 , j.
+  Proof.
+    rewrite /sstpk /sf_kind_sub/= /sf_star; iSplit; iIntros "/= #Hsub !>" (ρ).
+    iIntros (v) "#Hg".
+    by iDestruct ("Hsub" $! ρ with "Hg") as "{Hsub} (_ & #Hsub &_)"; iApply ("Hsub" $! v).
+    iIntros "#Hg"; repeat iSplit; iIntros "!>" (v); [iIntros "[]" | | iIntros "_ //"].
+    by iApply ("Hsub" $! ρ v with "Hg").
+  Qed.
+
+  Definition oTApp {n} (τ : oltyO Σ n.+1) (p : path) : olty Σ n :=
+    Olty (λ args ρ v, path_wp p.|[ρ] (λ w, vcurry τ w args ρ v)).
+End dot_types.
 End HkDot.
 
